ModularEngine/src/LogicEngine.FStar/infonlogic.fst
@@ -17,39 +17,7 @@ open Util
 open Subst
 open Typing
 open Unify
-
-(*********************************************************************************)
-(* Quotation prefixes *)
-(*********************************************************************************)
-logic function WithPrefix : prefix -> term -> term 
-assume forall (i:term). (WithPrefix [] i) = i
-assume forall (p:term) (pfx:prefix) (i:term). 
-  (WithPrefix (p::pfx) i) = (WithPrefix pfx (App SaidInfon [p; i]))
-val withPrefix: pfx:prefix -> i:term -> j:term{j=(WithPrefix pfx i)}
-let rec withPrefix pfx i = match pfx with 
-  | [] -> i
-  | p::pfx' -> (withPrefix pfx' (App SaidInfon [p; i]))
-
-(*********************************************************************************)
-(* Alpha conversion (for polyterms in infostrate) *)
-(*********************************************************************************)
-type alphaEquiv :: polyterm => polyterm => P =
-  | AEQ_Mono: i:term -> alphaEquiv (MonoTerm i) (MonoTerm i)
-
-  | AEQ_Poly: 
-       xs:vars -> t:term -> ys:vars
-    -> polytyping [] (ForallT xs t)
-    -> wfG ys 
-    -> varsTyEq xs ys
-    -> alphaEquiv (ForallT xs t) 
-                  (ForallT ys (Subst t (MkSubst xs (AsTerms ys))))
-
-  | AEQ_Justified: 
-      p:term -> i:polyterm -> d:term  -> j:polyterm
-    -> alphaEquiv i j 
-    -> alphaEquiv (JustifiedPoly p i d) (JustifiedPoly p j d)
-
-assume forall (i:polyterm) (j:polyterm). (CheckedInfon i && alphaEquiv i j) => CheckedInfon j
+open HilbertianQIL
 
 (* val checkVarsTyEq : xs:vars -> ys:vars -> option (varsTyEq xs ys) *)
 let checkVarsTyEq xs ys = zip_e<var, var, varTyEq> (fun x y -> (x.typ : typ)=y.typ) xs ys
@@ -86,103 +54,6 @@ let rec alphaConvert i = match i with
       let j = JustifiedPoly p q' d in 
         (j, AEQ_Justified p q d q' pf)
 
-
-  
-(*********************************************************************************)
-(* Definition of DKAL entailment *)
-(*********************************************************************************)
-type entails :: substrate => infostrate => vars => term => P =
-  | Entails_Emp : 
-       S:substrate -> K:infostrate -> G:vars
-    -> pref:prefix
-    -> typing G (WithPrefix pref (App EmptyInfon [])) Infon
-    -> entails S K G (WithPrefix pref (App EmptyInfon []))
-
-  | Entails_And_Intro : (* Simpler version with binary And *)
-       S:substrate -> K:infostrate -> G:vars
-    -> i:term -> j:term -> pref:prefix
-    -> entails S K G (WithPrefix pref i)
-    -> entails S K G (WithPrefix pref j)
-    -> entails S K G (WithPrefix pref (App AndInfon [i;j]))
-    
-  | Entails_And_Elim1 : 
-       S:substrate -> K:infostrate -> G:vars
-    -> i1:term -> i2:term -> pref:prefix
-    -> entails S K G (WithPrefix pref (App AndInfon [i1; i2]))
-    -> entails S K G (WithPrefix pref i1)
-    
-  | Entails_And_Elim2 : 
-       S:substrate -> K:infostrate -> G:vars
-    -> i1:term -> i2:term -> pref:prefix
-    -> entails S K G (WithPrefix pref (App AndInfon [i1; i2]))
-    -> entails S K G (WithPrefix pref i2)
-    
-  | Entails_W_Imp_Intro : 
-       S:substrate -> K:infostrate -> G:vars
-    -> i:term -> j:term -> pref:prefix
-    -> entails S K G (WithPrefix pref j)
-    -> typing G i Infon
-    -> entails S K G (WithPrefix pref (App ImpliesInfon [i; j]))
-
-  | Entails_Imp_Elim : 
-       S:substrate -> K:infostrate -> G:vars
-    -> i:term -> j:term -> pref:list term
-    -> entails S K G (WithPrefix pref i)
-    -> entails S K G (WithPrefix pref (App ImpliesInfon [i;j]))
-    -> entails S K G (WithPrefix pref j)
-
-  | Entails_Hyp_Substrate :
-       S:substrate -> K:infostrate -> G:vars
-    -> q:ISubstrateQueryTerm{SubstrateSays S q}     (* Eventually, we get a signature from the DB about this fact *)
-    -> entails S K G (App AsInfon [(SubstrateQueryTerm q)])
-
-  | Entails_Q_Elim:
-       S:substrate -> K:infostrate -> G:vars
-    -> xs:vars -> t:term -> is:list term 
-    -> polyentails S K G (ForallT xs t)
-    -> ZipP term var (fun (i:term) (x:var) => typing G i x.typ) is xs
-    -> entails S K G (Subst t (MkSubst xs is))
-
-  | Entails_J_Elim:
-       S:substrate -> K:infostrate -> G:vars
-    -> p:term -> i:term -> d:term -> pref:prefix
-    -> entails S K G (WithPrefix pref (App JustifiedInfon [p;i;d]))
-    -> entails S K G (WithPrefix pref i)
-
-  | Entails_Poly:
-       S:substrate -> K:infostrate -> G:vars
-    -> i:term
-    -> polyentails S K G (MonoTerm i)
-    -> entails S K G i
-
-and polyentails :: substrate => infostrate => vars => polyterm => P = 
-  | Entails_Hyp_Knowledge :
-       S:substrate -> K:infostrate -> G:vars
-    -> i:infon{In i K}
-    -> i':polyterm
-    -> polytyping [] i
-    -> alphaEquiv i i'
-    -> polytyping G i'
-    -> polyentails S K G i'
-
-  | Entails_Q_Intro :
-       S:substrate -> K:infostrate -> G:vars
-    -> i:term 
-    -> wfG G
-    -> entails S K G i 
-    -> polyentails S K [] (ForallT G i)
-
-  | Entails_Mono: 
-      S:substrate -> K:infostrate -> G:vars
-    -> i:term
-    -> entails S K G i
-    -> polyentails S K G (MonoTerm i)
-
-  | Entails_ElimJust: 
-      S:substrate -> K:infostrate -> G:vars
-    -> p:term -> i:polyterm -> d:term
-    -> polyentails S K G (JustifiedPoly p i d)
-    -> polyentails S K G i
 
 (*************************)
 (* Derivation algorithm  *)
