ModularEngine/src/LogicEngine.FStar/qil.fst
@@ -1,0 +1,203 @@
+(*
+// *********************************************************
+//
+//    Copyright (c) Microsoft. All rights reserved.
+//    This code is licensed under the Apache License, Version 2.0.
+//    THIS CODE IS PROVIDED *AS IS* WITHOUT WARRANTY OF
+//    ANY KIND, EITHER EXPRESS OR IMPLIED, INCLUDING ANY
+//    IMPLIED WARRANTIES OF FITNESS FOR A PARTICULAR
+//    PURPOSE, MERCHANTABILITY, OR NON-INFRINGEMENT.
+//
+// *********************************************************
+*)
+
+(* A complete, incremental decision procedure for quantified infon logic *)
+module QIL
+open Types
+open Util
+open Subst
+open Typing
+open Unify
+open HilbertianQIL
+
+(* TODO: Use a better implementation of sets of terms *)
+type set :: _ = list 
+let singleton x = [x]
+
+val setCons : 'a -> set 'a -> set 'a
+let setCons x y = 
+  if contains x y then y
+  else x::y
+
+val subformulas: term -> set term 
+let rec subformulas x = match x with 
+  | Var _ -> singleton x
+  | Const _ -> singleton x
+  | App AsInfon _ -> singleton x
+  | App EmptyInfon _ -> singleton x
+  | App (RelationInfon _) _ -> singleton x 
+  | App AndInfon args -> setCons x (collect subformulas args)
+  | App ImpliesInfon args -> setCons x (collect subformulas args)
+  | App SaidInfon [p; i] -> setCons x (map (fun j -> App SaidInfon [p; j]) (subformulas i))
+  | App JustifiedInfon [p; i; b] -> setCons x (subformulas i)
+  | _ -> raise "Unexpected infon form"
+
+type denv = {sf:set term; pfx:prefix; prins:set principal}
+
+type dterm :: _ = fun (pfx:prefix) (K:infostrate) =>
+    ((x:term * (S:substrate -> Partial (entails S K [] (WithPrefix pfx x)))))
+
+
+(* ******************************************************************************** *)
+(* Single-step derivations *)
+(* ******************************************************************************** *)
+val deriveAllOneStep : d:denv 
+              -> k:infostrate
+              -> from:list (dterm d.pfx k)
+              -> list (dterm d.pfx k)
+let deriveAllOneStep d k from = 
+  let pfx = d.pfx in 
+  let pairs : list (dterm pfx k) = product from from 
+    (fun (i, pfi) (j, pfj) -> 
+       let impElim =
+         match i with
+           | (App ImpliesInfon [i1;i2]) when j=i1 ->
+               let dt:dterm pfx k = 
+                 (i2, (fun s -> match pfi s, pfj s with 
+                         | MkPartial ei, MkPartial ej -> 
+                             MkPartial (Entails_Imp_Elim s k [] i1 i2 pfx ej ei))) in 
+                 ([dt] : list (dterm pfx k))
+           | _ -> [] in
+       let andIntro:dterm pfx k =
+         ((App AndInfon [i;j]),
+          (fun s -> bindP (pfi s) (fun ei ->
+                    mapP (pfj s) (fun ej -> 
+                         Entails_And_Intro s k [] i j pfx ei ej)))) in 
+         andIntro::impElim) in
+      
+    let singles : list (dterm pfx k) = coll from 
+      (fun (i, pfi) -> 
+         let andElim = match i with 
+           | App AndInfon [i1;i2] -> 
+               let dt1:dterm pfx k = 
+                 (i1, (fun s -> mapP (pfi s) (fun ei -> Entails_And_Elim1 s k [] i1 i2 pfx ei))) in 
+               let dt2:dterm pfx k = 
+                 (i2, (fun s -> mapP (pfi s) (fun ei -> Entails_And_Elim2 s k [] i1 i2 pfx ei))) in 
+                 [dt1;dt2]
+           | _ -> [] in 
+
+         let impIntro = coll d.sf
+           (fun phi -> match phi with 
+              | App ImpliesInfon [i1;i2] when i=i2 -> 
+                  let i1_t, i1_typing = doTyping [] i1 in 
+                    if i1_t = Infon then 
+                      let dt:dterm pfx k = 
+                        (phi, (fun s -> mapP (pfi s) (fun ei -> Entails_W_Imp_Intro s k [] i1 i2 pfx ei i1_typing))) in 
+                        [dt]
+                    else []
+              | _ -> []) in 
+
+         let jElim = match i with 
+           | App JustifiedInfon [p;i1;b] -> 
+               let dt:dterm pfx k = 
+                 (i1, (fun s -> mapP (pfi s) (fun ei -> Entails_J_Elim s k [] p i1 b pfx ei))) in 
+                 [dt]
+           | _ -> [] in 
+           
+           append andElim (append impIntro jElim)) in 
+
+    let axioms = from in 
+    let newones = append pairs singles in 
+    let _ = println (strcat "deriveOneStep with prefix " (string_of_any_for_coq pfx)) in
+    let _ = match newones with 
+      | [] -> println " derived nothing new"; ()
+      | _ -> iterate (fun i -> println (strcat "derived: " (string_of_any_for_coq i)); ()) newones in
+      (append pairs (append singles axioms) : list (dterm pfx k))
+
+(* ******************************************************************************** *)
+(* Boxing and unboxing quotations *)
+(* ******************************************************************************** *)
+val unbox:  p:term
+         -> pi:prefix 
+         -> k:infostrate
+         -> from:list (dterm pi k)
+         -> list (dterm (p::pi) k)
+let unbox p pfx k from = 
+  coll from (fun (i, pfi) -> match i with 
+                     | App SaidInfon [q; j] when p=q -> 
+                         let dt:dterm (p::pfx) k = (j,pfi) in 
+                           [dt]
+                     | _ -> [])
+
+val box: p:term
+      -> pfx:prefix
+      -> k:infostrate
+      -> from:list (dterm (p::pfx) k)  (* x where  (pfx (Said p x)) is derivable *)
+      -> list (dterm pfx k)            (* y=Said p x where  (pfx y) is derivable *)
+let box p pfx k from = coll from (fun (i, pfi) -> 
+                                    let dt:dterm pfx k = ((App SaidInfon [p;i]), pfi) in 
+                                      [dt])
+
+(* ******************************************************************************** *)
+(* Main derivation loop *)
+(* ******************************************************************************** *)
+val removeDups : list 'a -> ('a -> 'a -> bool) -> list 'a
+let rec removeDups l f = match l with 
+  | [] -> []
+  | hd::tl -> let res = removeDups tl f in 
+      if List_exists (fun hd' -> f hd hd') res
+      then res
+      else hd::res
+
+val setUnion : pfx:prefix -> k:infostrate 
+            -> list (dterm pfx k) 
+            -> list (dterm pfx k) 
+            -> list (dterm pfx k)
+let setUnion pfx k l1 l2 = 
+  removeDups (append l1 l2) (fun (i, _) (j, _) -> i=j)
+  
+val deriveAll:  d:denv 
+             -> k:infostrate 
+             -> list (dterm d.pfx k)
+             -> list (dterm d.pfx k)
+let rec deriveAll d k this_pfx = 
+  match this_pfx with 
+    | [] -> []
+    | _ -> 
+        let _ = println (strcat "deriveAll under pfx: " (string_of_any_for_coq d.pfx)) in 
+        let pre = setUnion d.pfx k 
+          (coll d.prins (fun pp -> 
+                     let p = Const (PrincipalConstant pp) in
+                     let this_p_pfx = unbox p d.pfx k this_pfx in 
+                     let next_p_pfx = deriveAll ({d with pfx=(p::d.pfx)}) k this_p_pfx in 
+                     let next_pfx : list (dterm d.pfx k) = box p d.pfx k next_p_pfx in
+                       next_pfx))
+          (deriveAllOneStep d k this_pfx) in 
+        let next_pfx = filter (fun ((i, pfi) : dterm d.pfx k) -> 
+                                 if contains ((withPrefix d.pfx i) : term) d.sf
+                                 then (println (strcat "Retaining " (string_of_any_for_coq i)); true)
+                                 else (println (strcat "Discarding " (string_of_any_for_coq i)); false)) pre in 
+          if (length next_pfx) = (length this_pfx) 
+          then next_pfx
+          else deriveAll d k next_pfx
+            
+
+val deriveAllWrapper: sf:list term 
+                   -> ps:list principal 
+                   -> k:infostrate 
+                   -> list (dterm [] k)
+let deriveAllWrapper sf ps k = 
+  let d = {sf=sf;
+           pfx=[];
+           prins=ps} in 
+  let dterm_hyp (i:infon{In i k}) : list (dterm d.pfx k) =     match i with 
+    | MonoTerm j -> 
+        match doPolyTyping [] i with 
+          | MkPartial pt -> 
+              let dt:dterm d.pfx k = 
+                (j, (fun s -> 
+                       MkPartial (Entails_Poly s k [] j
+                                    (Entails_Hyp_Knowledge s k [] i i pt (AEQ_Refl i) pt)))) in 
+                [dt] in 
+    deriveAll d k (collect_in k dterm_hyp)
+  
