ModularEngine/src/LogicEngine.FStar/testqil.fst
@@ -1,0 +1,55 @@
+module TestQIL
+open Types
+open QIL
+
+let said p i = App SaidInfon [(Const (PrincipalConstant p)); i]
+let implies i j = App ImpliesInfon [i;j]
+let andi i j = App AndInfon [i;j]
+let x = App (RelationInfon ({fname="X";
+                             retType=Infon;
+                             argsType=[];
+                             identity=None})) []
+
+let y = App (RelationInfon ({fname="Y";
+                             retType=Infon;
+                             argsType=[];
+                             identity=None})) []
+
+let bless i = 
+  map (fun (i:term) -> 
+         let j = MonoTerm i in 
+           assume (CheckedInfon j); 
+           (j:infon)) i
+
+val fst : 'a::* -> 'b::('a => *) -> (x:'a * 'b x) -> 'a
+let fst xy = let (x, _) = xy in x
+
+;; 
+
+  let infostrate = [(andi (said "p" x) (said "p" y))] in  
+  let sf = collect subformulas (append infostrate ([(said "p" (andi x y))])) in 
+  let _ = println "Got subformulas" in
+  let k = bless infostrate in 
+  let _ = println "Got infostrate ... go!" in
+  let facts = deriveAllWrapper sf ["p"; "q"; "r"] k in
+  let _ = println "All derivable facts: " in
+  let _ = iterate (fun (i : dterm [] k) -> let (j, _) = i in  println (string_of_any_for_coq j); ()) facts in
+     ()
+
+
+  (* let infostrate = [(said "p" (said "q" (implies (said "r" x) y))); *)
+  (*                   (said "p" (said "q" (said "r" x)))] in *)
+  (* let sf = collect subformulas infostrate in *)
+  (* let _ = println "Got subformulas" in  *)
+  (* let k = bless infostrate in *)
+  (* let _ = println "Got infostrate ... go!" in  *)
+  (* let facts = deriveAllWrapper sf ["p"; "q"; "r"] k in *)
+  (* let _ = println "All derivable facts: " inlet _ = iterate (fun (i : dterm [] k) -> let (j, _) = i in  println (string_of_any_for_coq j); ()) facts in  *)
+  (*    () *)
+
+
+
+
+
+                    
+
